Naming

Semantics/ReflTransRel.lean
@@ -1,37 +1,35 @@
 -- Reflexive transitive relations
-inductive RTL (r: α -> α -> Prop) (a: α): α -> Prop
-  | refl: RTL r a a
-  | tail: RTL r a b -> r b c -> RTL r a c
+inductive ReflTrans (r: α -> α -> Prop): α -> α -> Prop
+  | refl: ReflTrans r a a
+  | tail: ReflTrans r a b -> r b c -> ReflTrans r a c
 
-namespace RTL
+namespace ReflTrans
 
-theorem trans (hab: RTL r a b) (hbc: RTL r b c): RTL r a c:= by
+theorem trans (hab: ReflTrans r a b) (hbc: ReflTrans r b c): ReflTrans r a c := by
   induction hbc with
   | refl => exact hab
-  | tail _ hcd hac => exact hac.tail hcd
+  | tail _ hcd hac => exact tail hac hcd
 
-theorem single (hab: r a b): RTL r a b:=
-  refl.tail hab
+theorem single (hab: r a b): ReflTrans r a b :=
+  tail refl hab
 
-theorem head (hab: r a b) (hbc: RTL r b c): RTL r a c:= by
+theorem head (hab: r a b) (hbc: ReflTrans r b c): ReflTrans r a c := by
   induction hbc with
-  | refl => exact refl.tail hab
-  | tail _ hcd hac => exact hac.tail hcd
+  | refl => exact tail refl hab
+  | tail _ hcd hac => exact tail hac hcd
 
-theorem head_induction_on {P: ∀a: α, RTL r a b -> Prop} {a: α} (h: RTL r a b)
+theorem head_induction_on {P: ∀a: α, ReflTrans r a b -> Prop} {a: α} (h: ReflTrans r a b)
     (refl: P b refl)
-    (head: ∀{a c} (h': r a c) (h: RTL r c b), P c h -> P a (h.head h')): P a h:= by
+    (head: ∀{a c} (h': r a c) (h: ReflTrans r c b), P c h -> P a (head h' h)): P a h := by
   induction h with
   | refl => exact refl
   | tail _ hbc ih =>
-    apply ih
-    . exact head hbc _ refl
-    . exact fun h1 h2 => head h1 (h2.tail hbc)
+    exact ih (head hbc _ refl) (fun h1 h2 => head h1 (tail h2 hbc))
 
 theorem lift {r: α -> α -> Prop} {p: β -> β -> Prop} {a b: α} (f: α -> β)
-    (h: ∀{a b}, r a b -> p (f a) (f b)) (hab: RTL r a b): RTL p (f a) (f b):= by
+    (h: ∀{a b}, r a b -> p (f a) (f b)) (hab: ReflTrans r a b): ReflTrans p (f a) (f b) := by
   induction hab with
   | refl => exact refl
-  | tail _ hbc ih => exact ih.tail (h hbc)
+  | tail _ hbc ih => exact tail ih (h hbc)
 
-end RTL
+end ReflTrans
